some major changes everywhere + started proving termination of worklist

Machine.v
@@ -1,9 +1,13 @@
 (*Require Import Coq.FSets.FMaps.*)
-Require Import Coq.Lists.List.
+
 Require Import Coq.Program.Basics.
 Require Import Coq.Strings.String.
+Require Import Coq.Lists.List.
+Require Import Coq.Init.Logic.
+
 Require Import VerifiedVerifier.Bits.
 Require Import VerifiedVerifier.Maps.
+
 (*Require Import Coq.Vectors.Vector.*)
 (*Require Import SFI.Machine.Bits.*)
 (*Require Import bbv.Word.*)
@@ -70,7 +74,9 @@ Inductive conditional :=
 *)
 | Counter_Register_Zero.
 
-Inductive instr_class := 
+Definition label := nat.
+
+Inductive instr_class : Type := 
 | Heap_Read : register -> register -> register -> instr_class
 | Heap_Write : register -> register -> register -> instr_class
 | Heap_Check : register -> instr_class
@@ -81,21 +87,172 @@ Inductive instr_class :=
 | Stack_Contract : nat -> instr_class
 | Stack_Read : register -> nat -> instr_class
 | Stack_Write : nat -> register -> instr_class
+| Op : opcode -> list register -> list register -> instr_class
 | Indirect_Call : register -> instr_class
 | Direct_Call : string -> instr_class
-| Branch : conditional -> instr_class
-| Op : opcode -> list register -> list register -> instr_class
+| Branch : conditional -> label -> label -> instr_class
+| Jmp: label -> instr_class
 | Ret : instr_class.
+
+Definition terminating_instr_class i :=
+match i with
+| Branch _ _ _ | Jmp _ | Ret => true
+| _ => false
+end.
+
+Definition nonterminating_instr_class i :=
+negb (terminating_instr_class i). 
 
 Definition basic_block := list instr_class.
 
+Definition wf_instr_class (i : instr_class) (nodes : list basic_block) :=
+match i with
+| Branch _ t_label f_label => (t_label < length nodes) /\ (f_label < length nodes)
+| Jmp j_label => j_label < length nodes
+| Ret => True
+| _ => False
+end.
+
+Fixpoint wf_bb (bb : basic_block) (nodes : list basic_block) :=
+match bb with
+| i :: bb' => wf_instr_class i nodes /\ wf_bb bb' nodes
+| nil => True
+end.
+
+Structure ControlFlowGraph := {
+  V : list basic_block;
+  E : list (nat * nat);
+(*  E : list ({n : nat | n < length V} * {n : nat | n < length V}); *)
+  wf_cfg : forall bb, In bb V -> wf_bb bb V;
+}.
+
+
+
+(*
+
+Inductive terminating_instr_class : instr_class -> Prop :=
+| T_Branch: forall cond t_lable f_label,
+  terminating_instr_class (Branch cond t_lable f_label)
+| T_Jmp: forall j_label,
+  terminating_instr_class (Jmp j_label)
+| T_Ret:
+  terminating_instr_class (Ret).
+Hint Constructors terminating_instr_class.
+
+(*Definition branch_instr_class := {i : instr_class | forall cond t_label f_label, i = (Branch cond t_label f_label)}.
+Definition jmp_instr_class := {i : instr_class | forall j_label, i = (Jmp j_label)}.
+Definition ret_instr_class := {i : instr_class | i = (Ret)}.*)
+
+(* Definition term_instr_class := (sum branch_instr_class (sum jmp_instr_class ret_instr_class)). *)
+Definition term_instr_class := {i : instr_class | terminating_instr_class i}. 
+Definition nonterm_instr_class := {i : instr_class | not (terminating_instr_class i)}.
+(* Definition basic_block := {l : list instr_class | terminating_instr_class (last l)}. *)
+
+Inductive nonterminating_instr_class : instr_class -> Prop :=
+| NT_Heap_Read : forall r_dst r_src r_base,
+  nonterminating_instr_class (Heap_Read r_dst r_src r_base)
+| NT_Heap_Write: forall r_dst r_src r_base,
+  nonterminating_instr_class (Heap_Write r_dst r_src r_base)
+| NT_Heap_Check: forall reg,
+  nonterminating_instr_class (Heap_Check reg)
+| NT_Call_Check: forall reg,
+  nonterminating_instr_class (Call_Check reg)
+| NT_Reg_Move: forall r_dst r_src,
+  nonterminating_instr_class (Reg_Move r_dst r_src)
+| NT_Reg_Write: forall r_dst val,
+  nonterminating_instr_class (Reg_Write r_dst val)
+| NT_Stack_Expand: forall i,
+  nonterminating_instr_class (Stack_Expand i)
+| NT_Stack_Contract: forall i,
+  nonterminating_instr_class (Stack_Contract i)
+| NT_Stack_Read: forall r_dst i,
+  nonterminating_instr_class (Stack_Read r_dst i)
+| NT_Stack_Write: forall i r_src,
+  nonterminating_instr_class (Stack_Write i r_src)
+| NT_Indirect_Call: forall reg,
+  nonterminating_instr_class (Indirect_Call reg)
+| NT_Direct_Call: forall fname,
+  nonterminating_instr_class (Direct_Call fname)
+| NT_Op: forall op rs_dst rs_src,
+  nonterminating_instr_class (Op op rs_dst rs_src).
+Hint Constructors nonterminating_instr_class.
+
+Lemma instr_class_term_or_nonterm: forall i,
+  terminating_instr_class i \/ nonterminating_instr_class i.
+Proof.
+  destruct i; auto.
+Qed.
+
+Lemma instr_class_not_term_and_nonterm: forall i,
+  ~ (terminating_instr_class i /\ nonterminating_instr_class i).
+Proof.
+  destruct i; intros H; inversion H; try inversion H0; try inversion H1.
+Qed.
+
+Inductive basic_block' : Type:=
+| Basic_Block_One: 
+  term_instr_class -> basic_block'
+| Basic_Block_Many:
+  nonterm_instr_class -> basic_block' -> basic_block'.
+
+Fixpoint last (bb : basic_block') : term_instr_class :=
+match bb with
+| Basic_Block_One i => i
+| Basic_Block_Many i bb' => last bb'
+end.
+
+Program Definition branch_block := {bb : basic_block' | forall cond t_label f_label, last bb = (Branch cond t_label f_label)}.
+Program Definition jmp_block := {bb : basic_block' | forall j_label, last bb = (Jmp j_label)}.
+Program Definition ret_block := {bb : basic_block' | last bb = Ret}.
+
+Definition basic_block := branch_block + jmp_block + ret_block.
+
+Definition bb_last (bb : basic_block) : term_instr_class :=
+match bb with
+| inl (inl branch) => last (proj1_sig branch)
+| inl (inr jmp) => last (proj1_sig jmp)
+| inr ret => last (proj1_sig ret)
+end.
+
+Definition wf_bb (bb : basic_block) (nodes : list basic_block) :=
+match proj1_sig (bb_last bb) with
+| Branch _ t_label f_label => (t_label < length nodes) /\ (f_label < length nodes)
+| Jmp j_label => j_label < length nodes
+| Ret => True
+| _ => False
+end.
+
+Structure ControlFlowGraph := {
+  V : list basic_block;
+  E : list ({src : basic_block | In src V} * {dst : basic_block | In dst V});
+  wf_cfg : forall bb, In bb V -> wf_bb bb V;
+}.
+*)
+
+Definition function := ControlFlowGraph.
+
+Definition program := list ControlFlowGraph.
+
+(* Definition basic_block := list instr_class. *)
+(*
 Inductive edge_class : Set :=
 | True_Branch
 | False_Branch
 | Non_Branch.
 
-Definition node_ty := prod basic_block nat.
+Compute (head (1 :: 2 :: nil)).
+
+
+Definition node_ty := prod label basic_block.
 Definition edge_ty := (prod (prod node_ty node_ty) edge_class).
+
+Structure DiGraph := {
+  V :> nat ; (* The number of vertices. So the vertices are numbers 0, 1, ..., V-1. *)
+  E :> nat -> nat -> Prop ; (* The edge relation *)
+  E_decidable : forall x y : nat, ({E x y} + {~ E x y}) ;
+}.
+
+Definition cfg
 
 Record cfg_ty := {
   nodes : list node_ty;
@@ -124,6 +281,9 @@ Definition edges_in_nodes (cfg : cfg_ty) : Prop :=
 (* TODO: This definition is incomplete *)
 Definition well_formed_cfg (cfg : cfg_ty) : Prop :=
   unique_bb cfg /\ edges_in_nodes cfg.
+*)
+
+
 
 Definition well_formed_fun (f : function_ty) : Prop :=
   well_formed_cfg (fst f).
@@ -147,10 +307,11 @@ Definition conditional_eq_dec : forall (x y : conditional), {x=y} + {x<>y}.
   intros; decide equality; try apply register_eq_dec.
 Defined.
 
+(*
 Definition edge_class_eq_dec : forall (x y : edge_class), {x=y} + {x<>y}.
   intros; decide equality.
 Defined.
-
+*)
 Definition value_eq_dec : forall (x y: value), {x=y} + {x<>y}.
   intros; decide equality; try apply register_eq_dec; try apply int64_eq_dec.
 Defined.
@@ -160,6 +321,7 @@ Definition instr_class_eq_dec : forall (x y : instr_class), {x=y} + {x<>y}.
   try apply conditional_eq_dec; decide equality; decide equality.
 Defined.
 
+(*
 Definition basic_block_eq_dec : forall (x y : basic_block), {x=y} + {x<>y}.
   intros; decide equality; apply instr_class_eq_dec.
 Defined.
@@ -189,7 +351,7 @@ Definition edge_ty_eqb (a : edge_ty) (b : edge_ty) : bool :=
   if edge_ty_eq_dec a b
   then true
   else false.
-
+*)
 Inductive flag : Set :=
 | of
 | sf
