AbstractAnalysis.v
@@ -2,8 +2,8 @@ Require Import VerifiedVerifier.Machine.
 Require Import VerifiedVerifier.BoundedLattice.
 Require Import VerifiedVerifier.BinaryLattice.
 Require Import VerifiedVerifier.Maps.
-Require Import Coq.Lists.List.
 Require Import Coq.Init.Nat.
+Require Import Coq.Lists.List.
 
 Record info := {
   abs_heap_base : BinarySet;
@@ -11,12 +11,12 @@ Record info := {
   abs_cf_bound : BinarySet;
 }.
 
-Definition empty_info :=
+Definition top_info :=
   {| abs_heap_base := top;
      abs_heap_bound := top;
      abs_cf_bound := top; |}.
 
-Definition bottom_info :=
+Definition bot_info :=
   {| abs_heap_base := bottom;
      abs_heap_bound := bottom;
      abs_cf_bound := bottom; |}.
@@ -40,77 +40,131 @@ Definition abs_registers_ty := total_map register info.
 
 Definition abs_stack_ty := list info.
 
-Record abs_state := {
+Record abs_state' := {
   abs_regs : abs_registers_ty;
 (*  flags : flags_ty; *)
   abs_stack : abs_stack_ty;
-  abs_error : bool;
+(*  abs_error : bool; *)
 }.
 
-Definition abs_state_eq_dec : forall (x y : abs_state), {x=y} + {x<>y}.
+Inductive abs_state :=
+| top_state : abs_state
+| bot_state : abs_state
+| sub_state : abs_state' -> abs_state.
+
+Definition abs_state'_eq_dec : forall (x y : abs_state'), {x=y} + {x<>y}.
 intros x y. decide equality; subst; try decide equality; try decide equality; try decide equality.
 admit. (* funcational extensionality we can get rid of making this an axiim if we use a different implementation of map *)
 Admitted.
+
+Definition abs_state_eq_dec : forall (x y : abs_state), {x=y} + {x<>y}.
+intros x y; decide equality; apply abs_state'_eq_dec.
+Qed.
 
 Definition abs_state_eqb (a : abs_state) (b : abs_state) : bool :=
   if abs_state_eq_dec a b
   then true
   else false.
 
-Definition abs_empty_state :=
-{| abs_regs := fun r => if register_eq_dec r rdi
+Definition abs_top_state := top_state.
+(* {| abs_regs := fun r => if register_eq_dec r rdi
                           then abs_heap_base_info
                           else empty_info;
    abs_stack := nil;
-   abs_error := false; |}.
+   abs_error := false; |}. *)
 
-Definition abs_bottom_state :=
-{| abs_regs := t_empty bottom_info;
+Definition abs_bot_state := bot_state.
+(* {| abs_regs := t_empty bottom_info;
    abs_stack := nil;
-   abs_error := false; |}.
+   abs_error := false; |}. *)
 
-Definition expand_abs_stack (s : abs_state) (i : nat) : abs_state :=
-{| abs_regs := s.(abs_regs);
-(*   flags := s.(flags); *)
-   abs_stack := s.(abs_stack) ++ (repeat empty_info i);
-   abs_error := s.(abs_error); |}.
+Definition init_state' :=
+ {| abs_regs := fun r => if register_eq_dec r rdi
+                          then abs_heap_base_info
+                          else top_info;
+   abs_stack := nil; |}.
 
-Fixpoint contract_abs_stack (s : abs_state) (i : nat) : abs_state :=
-match i with
-| 0 => s
-| S n =>
-contract_abs_stack {| abs_regs := s.(abs_regs);
-(*   flags := s.(flags); *)
-   abs_stack := removelast s.(abs_stack);
-   abs_error := s.(abs_error); |} n
-end.
+Definition init_state := sub_state init_state'.
 
-Definition get_register_info (s : abs_state) (r : register) : info :=
+Definition expand_abs_stack (s : abs_state') (i : nat) : abs_state' :=
+ {| abs_regs := s.(abs_regs);
+    abs_stack := s.(abs_stack) ++ (repeat top_info i); |}.
+
+Fixpoint contract_abs_stack (s : abs_state') (i : nat) : abs_state' :=
+  match i with
+  | 0 => s
+  | S n =>
+    contract_abs_stack {| abs_regs := s.(abs_regs);
+                                     abs_stack := removelast s.(abs_stack) |} n
+  end.
+
+Definition get_register_info (s : abs_state') (r : register) : info :=
   s.(abs_regs) r.
 
-Definition set_register_info (s : abs_state) (r : register) (i : info) : abs_state :=
+Definition set_register_info (s : abs_state') (r : register) (i : info) : abs_state' :=
 {| abs_regs := t_update register_eq_dec s.(abs_regs) r i;
-   abs_stack := s.(abs_stack);
-   abs_error := s.(abs_error); |}.
+   abs_stack := s.(abs_stack); |}.
+
+Definition clear_registers_info (s : abs_state') : abs_state' :=
+{| abs_regs := (fun _ => top_info) ;
+   abs_stack := s.(abs_stack); |}.
+
 
 (* TODO: make stack indexing 64-bit *)
-Definition get_stack_info (s : abs_state) (index : nat) : info :=
-nth index s.(abs_stack) empty_info.
+Definition get_stack_info (s : abs_state') (index : nat) : info :=
+nth index s.(abs_stack) top_info.
 
 (* this needs to be updated *)
-Definition set_stack_info (s : abs_state) (index : nat) (i : info) : abs_state :=
+Definition set_stack_info (s : abs_state') (index : nat) (i : info) : abs_state' :=
 {| abs_regs := s.(abs_regs);
-   abs_stack := Machine.update s.(abs_stack) index i;
-   abs_error := s.(abs_error); |}.
+   abs_stack := Machine.update s.(abs_stack) index i; |}.
 
+(*
 Definition is_abs_error (s : abs_state) : bool :=
   s.(abs_error).
+
 
 Definition set_error_state (s : abs_state) : abs_state :=
 {| abs_regs := s.(abs_regs);
    abs_stack := s.(abs_stack);
    abs_error := true; |}.
+*)
 
+Definition join_info (i1 : info) (i2 : info) : info :=
+{| abs_heap_base := join_BinarySet i1.(abs_heap_base) i2.(abs_heap_base);
+   abs_heap_bound := join_BinarySet i1.(abs_heap_bound) i2.(abs_heap_bound);
+   abs_cf_bound := join_BinarySet i1.(abs_cf_bound) i2.(abs_cf_bound); |}.
+
+Definition join_abs_regs (r1 : abs_registers_ty) (r2 : abs_registers_ty) : abs_registers_ty :=
+  fun r => join_info (r1 r) (r2 r).
+
+Fixpoint join_abs_stack (s1 : abs_stack_ty) (s2 : abs_stack_ty) : abs_stack_ty :=
+  match s1 with
+  | i1 :: s1' =>
+    match s2 with
+    | i2 :: s2' => join_info i1 i2 :: join_abs_stack s1' s2'
+    | _ => nil
+    end
+  | _ => nil
+  end.
+
+Definition join_abs_state' (s1 : abs_state') (s2 : abs_state') : abs_state' :=
+{| abs_regs := join_abs_regs s1.(abs_regs) s2.(abs_regs);
+   abs_stack := join_abs_stack s1.(abs_stack) s2.(abs_stack); |}.
+
+Definition join_abs_state (s1 : abs_state) (s2 : abs_state) : abs_state :=
+match s1, s2 with
+| top_state, _ | _, top_state => top_state
+| sub_state s1', sub_state s2' => if (abs_state'_eq_dec s1' s2') then sub_state s1' else top_state
+| sub_state s1', _ => sub_state s1'
+| _, sub_state s2' => sub_state s2'
+| _, _ => bot_state
+end.
+
+Fixpoint join_abs_states (ss : list abs_state) : abs_state :=
+  fold_left join_abs_state ss bot_state.
+
+(*
 Definition meet_info (i1 : info) (i2 : info) : info :=
 {| abs_heap_base := meet_BinarySet i1.(abs_heap_base) i2.(abs_heap_base);
    abs_heap_bound := meet_BinarySet i1.(abs_heap_bound) i2.(abs_heap_bound);
@@ -132,12 +186,19 @@ Fixpoint meet_abs_stack (s1 : abs_stack_ty) (s2 : abs_stack_ty) : abs_stack_ty :
   | _ => nil
   end.
 
-Definition meet_abs_state (s1 : abs_state) (s2 : abs_state) : abs_state :=
+Definition meet_abs_state' (s1 : abs_state') (s2 : abs_state') : abs_state' :=
 {| abs_regs := meet_abs_regs s1.(abs_regs) s2.(abs_regs);
-   abs_stack := meet_abs_stack s1.(abs_stack) s2.(abs_stack);
-   abs_error := orb (orb s1.(abs_error) s2.(abs_error))
-                    (negb (eqb (length s1.(abs_stack)) (length s2.(abs_stack))));
-|}.
+   abs_stack := meet_abs_stack s1.(abs_stack) s2.(abs_stack); |}.
+
+
+Definition meet_abs_state (s1 : abs_state) (s2 : abs_state) : abs_state :=
+match s1 with
+| bot_state => bot_state
+| 
+{| abs_regs := meet_abs_regs s1.(abs_regs) s2.(abs_regs);
+   abs_stack := meet_abs_stack s1.(abs_stack) s2.(abs_stack); |}.
+
+
 
 (* TODO: need to add a bottom state; currently abs_bottom_state has a stack
  * of length 0, which means that meet_abs_state will return an error state
@@ -147,6 +208,7 @@ Fixpoint meet_abs_states (ss : list abs_state) : abs_state :=
   | s :: ss' => meet_abs_state s (meet_abs_states ss')
   | _ => abs_bottom_state
   end.
+
 
 Fixpoint get_parent_nodes (n : node_ty) (es : list edge_ty) : list node_ty :=
   match es with
@@ -180,16 +242,197 @@ Definition empty {A} (l : list A) :=
 
 Definition initialize_worklist (cfg : cfg_ty) : total_map node_ty abs_state :=
   t_empty abs_empty_state.
-
+*)
 (* TODO: Add check instructions for everything else *)
 Reserved Notation " i '/' st 'v-->' st' "
                   (at level 40, st' at level 39).
-Inductive instr_class_vstep : instr_class -> abs_state -> abs_state -> Prop := 
+
+Definition instr_class_flow_function (i : instr_class) (s : abs_state') : abs_state' :=
+match i with 
+| Heap_Read r_dst _ _ => set_register_info s r_dst top_info
+| Heap_Write _ _ _ => s
+| Heap_Check r_src => set_register_info s r_src abs_heap_bounded_info
+| Call_Check r_src => set_register_info s r_src abs_cf_bounded_info
+| Reg_Move r_dst r_src => set_register_info s r_dst (get_register_info s r_src)
+| Reg_Write r_dst _ => set_register_info s r_dst top_info
+| Stack_Expand i => expand_abs_stack s i
+| Stack_Contract i => contract_abs_stack s i
+| Stack_Read r_dst i => set_register_info s r_dst (get_stack_info s i)
+| Stack_Write i r_src => set_stack_info s i (get_register_info s r_src)
+| Op op rs_dst rs_src => fold_left (fun s r => set_register_info s r top_info) rs_dst s
+| Indirect_Call reg => clear_registers_info s
+| Direct_Call fname => clear_registers_info s
+| Branch _ _ _ => s
+| Jmp _ => s
+| Ret => s
+end.
+
+Fixpoint basic_block_flow_function (bb : basic_block) (s : abs_state) : abs_state :=
+match bb with
+| nil => s
+| i :: bb' => 
+  match s with
+  | top_state => top_state
+  | bot_state => bot_state
+  | sub_state s' => basic_block_flow_function bb' (sub_state (instr_class_flow_function i s'))
+  end
+end.
+
+Fixpoint map2 {A B C} (f : A -> B -> C) (aa : list A) (bb : list B) : list C :=
+match aa, bb with
+| a :: aa', b :: bb' => (f a b) :: (map2 f aa' bb')
+| _, _ => nil
+end.
+
+Fixpoint eq_list (l1 : list abs_state) (l2 : list abs_state) : bool :=
+match l1, l2 with 
+| nil, nil => true
+| a :: aa, b :: bb => andb (abs_state_eqb a b) (eq_list aa bb)
+| _, _ => false
+end.
+
+Fixpoint get_incoming_edges (E: list (nat * nat) ) (i : nat) :=
+match E with
+| nil => nil
+| (src, dst) :: E' => 
+  let incoming_edges := get_incoming_edges E' i in
+  if (eqb i dst) then src :: incoming_edges else incoming_edges 
+end.  
+
+Fixpoint get_outgoing_edges (E: list (nat * nat) ) (i : nat) :=
+match E with
+| nil => nil
+| (src, dst) :: E' => 
+  let incoming_edges := get_incoming_edges E' i in
+  if (eqb i src) then dst :: incoming_edges else incoming_edges 
+end.
+
+Definition nth_state (n : nat) (l : list abs_state) :=
+nth n l bot_state.
+
+Definition nth_block (n : nat) (l : list basic_block) :=
+nth n l nil.
+
+Require Import FunInd.
+Require Import Recdef.
+
+Inductive leq_info : info -> info -> Prop :=
+| leq_info_refl : forall i,
+  leq_info i i
+| leq_info_rule : forall x y,
+  BinaryRel (abs_heap_base x) (abs_heap_base y) ->
+  BinaryRel (abs_heap_bound x) (abs_heap_bound y) ->
+  BinaryRel (abs_cf_bound x) (abs_cf_bound y) ->
+  leq_info x y.
+
+Inductive leq_abs_state' : abs_state' -> abs_state' -> Prop :=
+| leq_abs_state'_rule: forall st st',
+  (forall reg, leq_info (get_register_info st reg) (get_register_info st' reg)) ->
+  (forall i, leq_info (get_stack_info st i) (get_stack_info st' i)) -> 
+  length (abs_stack st) = length (abs_stack st') ->
+  leq_abs_state' st st'.
+
+Inductive leq_abs_state : abs_state -> abs_state -> Prop :=
+| leq_bot_state: forall s, 
+  leq_abs_state bot_state s
+| leq_top_state: forall s, 
+  leq_abs_state s top_state
+| leq_sub_state: forall s1 s2,
+  leq_abs_state' s1 s2 ->
+  leq_abs_state (sub_state s1) (sub_state s2).
+
+Definition ge_abs_state s1 s2 := leq_abs_state s2 s1.
+
+Inductive ge_abs_states : list abs_state -> list abs_state -> Prop :=
+| ge_abs_states_nil: 
+  ge_abs_states nil nil
+| ge_abs_states_cons: forall s1 s2 ss1 ss2,
+  ge_abs_state s1 s2 ->
+  ge_abs_states ss1 ss2 ->
+  ge_abs_states (s1 :: ss1) (s2 :: ss2).
+
+Require Import Recdef.
+
+(*Function div2_Fun (n:nat)
+        {wf lt }
+        : nat :=
+match n with
+| S (S k) => S (div2_Fun k)
+| _ => 0
+end.*)
+
+Function worklist' (queue : list nat) (f : function) (ss : list abs_state) { wf ge_abs_states ss } : list abs_state :=
+match queue with
+| nil => ss
+| i :: queue' => 
+  let in_edges := get_incoming_edges (E f) i in
+  let in_states := map (fun i => nth_state i ss) in_edges in
+  let in_state := join_abs_states in_states in
+  let out_state := basic_block_flow_function (nth_block i (V f)) in_state in 
+  let out_edges := get_outgoing_edges (E f) i in
+  let updated_edges := filter (fun i => abs_state_eqb (nth_state i ss) out_state) out_edges in
+  let new_queue := queue' ++ updated_edges in
+  let new_ss := fold_left (fun ss' i' => Machine.update ss' i' (join_abs_state (nth_state i ss') out_state)) updated_edges ss in
+  worklist' new_queue f new_ss
+end.
+Proof.
+Admitted.
+
+Fixpoint worklist (f : function) (ss : list abs_state) : list abs_state :=
+  worklist' (seq 0 (length f)) f ss.
+
+Definition greatest_fixpoint (f: function) : list abs_state :=  
+worklist f ((init_state :: nil) ++ (repeat bot_state (length (V f) - 1))).
+
+Definition instr_class_verifier (i : instr_class) (s : abs_state') : Prop :=
+(* I'm not sure what the right implementation is here *)
+(* we might need to add a match for every top=>false bot=>true *)
+  match i with
+  | Heap_Read _ r_src r_base => 
+    (get_register_info s r_base).(abs_heap_base) = bottom /\ (get_register_info s r_src).(abs_heap_bound) = bottom
+  | Heap_Write r_dst _ r_base =>
+    (get_register_info s r_base).(abs_heap_base) = bottom /\ (get_register_info s r_dst).(abs_heap_bound) = bottom
+  | Stack_Contract i =>
+    i <= (length s.(abs_stack))
+  | Stack_Read _ i =>
+    i < (length s.(abs_stack))
+  | Stack_Write i _ =>
+    i < (length s.(abs_stack))
+  | Indirect_Call reg =>
+    (get_register_info s reg).(abs_cf_bound) = bottom /\ (get_register_info s rdi).(abs_heap_base) = bottom
+  | Direct_Call fname =>
+    (get_register_info s rdi).(abs_heap_base) = bottom (* TODO: do we need to check that the function name is defined *)
+  | Ret =>
+    length s.(abs_stack) = 0
+  | _ => True
+end.
+
+Fixpoint basic_block_verifier (bb : basic_block) (s : abs_state) : Prop :=
+match bb with
+| nil => True
+| i :: bb' => 
+  match s with
+  | top_state => False
+  | bot_state => True
+  | sub_state s' => instr_class_verifier i s' /\ basic_block_verifier bb' (sub_state (instr_class_flow_function i s'))
+  end
+end.
+
+(*
+Definition function_verifier (f : function) : Prop :=
+Forall2 basic_block_verifier (f.V) (greatest_fixpoint f).
+
+Definition program_verifier (p : program) : Prop :=
+Forall function_verifier p.
+*)
+
+(*
+Inductive instr_class_vstep : instr_class -> abs_state' -> abs_state' -> Prop := 
 | V_Heap_Read: forall st r_base r_src r_dst,
     (* r_base <> r_src -> *) (* not sure if we need this to make the proofs easier *)
     (get_register_info st r_base).(abs_heap_base) = bottom ->
     (get_register_info st r_src).(abs_heap_bound) = bottom ->
-    Heap_Read r_dst r_src r_base / st v--> (set_register_info st r_dst empty_info) 
+    Heap_Read r_dst r_src r_base / st v--> (set_register_info st r_dst top_info) 
 | V_Heap_Write: forall st r_base r_src r_dst,
     (* r_base <> r_src -> *) (* not sure if we need this to make the proofs easier *)
     (get_register_info st r_base).(abs_heap_base) = bottom ->
@@ -202,7 +445,7 @@ Inductive instr_class_vstep : instr_class -> abs_state -> abs_state -> Prop :=
 | V_Reg_Move: forall st r_src r_dst,
     Reg_Move r_dst r_src / st v--> (set_register_info st r_dst (get_register_info st r_src))
 | V_Reg_Write: forall st r_dst val,
-    Reg_Write r_dst val / st v--> (set_register_info st r_dst empty_info)
+    Reg_Write r_dst val / st v--> (set_register_info st r_dst top_info)
 | V_Stack_Expand: forall st i,
     Stack_Expand i / st v--> (expand_abs_stack st i)
 | V_Stack_Contract: forall st i,
@@ -214,6 +457,8 @@ Inductive instr_class_vstep : instr_class -> abs_state -> abs_state -> Prop :=
 | V_Stack_Write: forall st i r_src,
     i < (length st.(abs_stack)) ->
     Stack_Write i r_src / st v--> (set_stack_info st i (get_register_info st r_src))
+| V_Op: forall st op rs_dst rs_src,
+    Op op rs_dst rs_src / st v--> fold_left (fun s r => set_register_info s r top_info) rs_dst st
 | V_Indirect_Call: forall st reg,
     (get_register_info st reg).(abs_cf_bound) = bottom ->
     (get_register_info st rdi).(abs_heap_base) = bottom ->
@@ -221,12 +466,12 @@ Inductive instr_class_vstep : instr_class -> abs_state -> abs_state -> Prop :=
 | V_Direct_Call: forall st str,
     (get_register_info st rdi).(abs_heap_base) = bottom ->
     Direct_Call str / st v-->  st
-| V_Branch: forall st cond, 
-    Branch cond / st v--> st
-| V_Op: forall st op rs_dst rs_src,
-    Op op rs_dst rs_src / st v--> fold_left (fun s r => set_register_info s r empty_info) rs_dst st
+| V_Branch: forall st cond t_label f_label, 
+    Branch cond t_label f_label / st v--> st
+| V_Jmp: forall st j_label,
+    Jmp j_label / st v--> st
 | V_Ret: forall st,
-    empty st.(abs_stack) ->
+    length st.(abs_stack) = 0 ->
     Ret / st v-->  st
   where " i '/' st 'v-->' st'" := (instr_class_vstep i st st').
 Hint Constructors instr_class_vstep.
@@ -278,7 +523,7 @@ Definition flow_function (st : abs_state) (i : instr_class) : abs_state :=
 
 Fixpoint bb_flow_function (st : abs_state) (bb : basic_block) : abs_state :=
   match bb with
-  | i :: bb' => bb_flow_function (flow_function st i) bb'
+  | i :: bb' => bb_flow_function (instr_class_flow_function st i) bb'
   | _ => st
   end.
 
@@ -381,3 +626,4 @@ Proof.
     + unfold get_register_info in *. unfold set_register_info. simpl.
       rewrite register_get_after_set_eq; auto.
 Qed.
+*)
